michael_formal/Filesystem.thy
@@ -34,7 +34,7 @@ definition "write" :: "transition" where
         Arity = 1,
         Guard = [], (* No guards *)
         Outputs = [],
-        Updates = [ (* Two updates: *)
+        Updates = [ 
                     (''r1'', (V ''r1'')), (* Value of r1 remains unchanged *)
                     (''r2'', (V ''i1'')), (* Write the input to r2 *)
                     (''r3'', (V ''r1''))  (* Store the writer in r3 *)
@@ -89,14 +89,31 @@ primrec all :: "'a list \<Rightarrow> ('a \<Rightarrow> bool) \<Rightarrow> bool
 
 (* noChangeOwner: THEOREM filesystem |- G(cfstate /= NULL_STATE) => FORALL (owner : UID): G((label=write AND r_1=owner) => F(G((label=read AND r_1/=owner) => X(op_1_read_0 = accessDenied)))); *)
 
-lemma "x \<noteq> ''r1'' \<longrightarrow> x \<noteq> ''r3'' \<longrightarrow> x \<noteq> ''r2'' \<longrightarrow> r x = 0 \<Longrightarrow> r ''r3'' \<noteq> r ''r1'' \<Longrightarrow> step filesystem 2 r ''read'' [] = Some (2, [0], r)"
-  apply (simp add: fs_simp step_def join_def null_state_def)
-  apply (rule ext)
-  apply simp
-  
-  
+lemma aux_write: "concat (map (\<lambda>s'. concat (map (\<lambda>t. if Label t = ''write'' \<and>
+                                                 (\<exists>y. find (\<lambda>x. x = t) (T filesystem (2, s')) = Some y) \<and>
+                                                 Suc 0 = Arity t \<and> apply_guards (Guard t) (\<lambda>x. if x = index 1 then content else join_ir [] r (1 + 1) x) r
+                                              then [(s', t)] else [])
+                                      (T filesystem (2, s'))))
+                   (S filesystem)) = [(2, write)]"
+  by (simp add: fs_simp)
 
-lemma "(r ''r3'' \<noteq> r ''r1'') \<Longrightarrow> all (observe_trace filesystem 2 r t) (\<lambda>e. e = [] \<or> e = [0])"
+lemma joinir: "(\<lambda>x. if x = index 1 then content else join_ir [] r (1 + 1) x) = (\<lambda>x. if x = ''i1'' then content else r x)"
+  apply (rule ext)
+  by (simp add: index_def shows_stuff)
+
+lemma aux1: "(r ''r3'' \<noteq> r ''r1'') \<Longrightarrow> step filesystem 2 r ''read'' [] = Some (2, [0], r)"
+  apply (simp add: fs_simp step_def index_def shows_stuff join_def)
+  apply (rule ext)
+  by simp
+
+lemma aux2: "step filesystem 2 r ''write'' [content] = Some (2, [], (\<lambda>x. if x = ''r1'' \<or> x = ''r3'' then r ''r1'' else (if x = ''r2'' then content else r x)))"
+  apply (simp add: step_def aux_write)
+  apply safe
+   apply (simp add: write_def)
+  apply (rule ext)
+  by (simp add: joinir write_def)
+
+lemma "(r ''r3'' \<noteq> r ''r1'') \<Longrightarrow> valid_trace filesystem t \<Longrightarrow> all (observe_trace filesystem 2 r t) (\<lambda>e. e = [] \<or> e = [0])"
 proof (induction t)
   case Nil
   then show ?case by simp
@@ -109,7 +126,13 @@ next
     apply simp
     apply safe
     apply (cases "a = (''read'', [])")
+     apply (simp add: aux1)
+     apply (cases "a = (''write'', [content])")
     apply simp
+      apply (simp add: aux2)
+    
+
+
 
 qed
 
